Java/src/Java/Tactics/FieldLookup.v
@@ -1,0 +1,115 @@
+Require Import MirrorCore.RTac.Core.
+Require Import MirrorCore.Lambda.Expr.
+Require Import MirrorCore.Lambda.ExprUnify_simul.
+
+Require Import Java.Func.JavaFunc.
+Require Import Java.Func.JavaType.
+Require Import Java.Language.Program.
+
+Require Import Charge.ModularFunc.BaseFunc.
+
+Section FieldLookup.
+  Context {fs : Environment}.
+
+  Definition FIELD_LOOKUP : rtac typ (expr typ func) :=
+	fun tus tvs n m c s e =>
+		match e with
+		  | App (App (App (Inj (inr pMethodLookup)) (pProg P)) C) f =>
+		    match baseS C with
+		      | Some (pConst tyString C') =>
+				match class_lookup C' P with
+		    	  | Some Class =>
+		    	    match @exprUnify (ctx_subst c) typ func _ _ _ _ _ 3
+		                             tus tvs 0 f (mkFields (c_fields Class)) tyVarList s with
+		              | Some s => Solved s
+		              | None   => Fail
+		            end
+				  | _ => Fail
+				end
+			  | _ => Fail
+			end
+		  | _ => Fail
+		end.
+(*
+Lemma FIELD_LOOKUP_sound : rtac_sound FIELD_LOOKUP.
+Proof.
+  unfold rtac_sound, rtac_spec; intros.
+  unfold FIELD_LOOKUP, fieldLookupTac in H.
+  destruct g; subst; try apply I.
+  forward.
+  simpl in H10.
+  forward.
+  SearchAbout exprUnify'.
+  Print exprUnify'.
+  Print ExprUnify_common.unify_sound_ind.
+  pose proof (exprUnify_sound).
+  specialize(H13 (ctx_subst ctx) typ func _ _ _ _ _ _ _ _ _ _ 3).
+  red in H13.
+  red in H13.
+  apply H13 with (tv' := nil) in H10; clear H13; [|assumption].
+  forward_reason; split; auto.
+  forward. simpl in H13.
+  simpl in H15.
+  unfold Ctx.propD, exprD'_typ0 in H15.
+  forward; inv_all; subst.
+  simpl in H15.
+  autorewrite with exprD_rw in H15; [|apply _];
+  simpl in H15; forward; inv_all; subst.
+  autorewrite with exprD_rw in H0.
+  simpl in H0; forward; inv_all; subst.
+  autorewrite with exprD_rw in H2; [|apply _];
+  simpl in H2; forward; inv_all; subst.
+  autorewrite with exprD_rw in H2; [|apply _];
+  simpl in H2; forward; inv_all; subst.
+  unfold funcAs in H2. simpl in H2.
+  forward; inv_all; subst.
+  pose proof (pctxD_substD H12 H14).
+  destruct H as [? [? ?]].
+  specialize (H13 _ _ _ H5 eq_refl H).
+  forward; inv_all; subst.
+  destruct H6 as [? [? ?]].
+  pose proof (substD_pctxD _ H10 H14 H6).
+  destruct H13 as [? [? ?]].
+  simpl in *. unfold Expr_expr.
+  rewrite H13.
+  split. admit.
+  intros. unfold exprT_App, exprT_Inj in *; simpl in *.
+  destruct e0; inv_all; try congruence.
+  destruct f; try congruence.
+  destruct s1; try congruence.
+  destruct s1; try congruence.
+  destruct s1; try congruence.
+  destruct s1; try congruence.
+  destruct s1; try congruence.
+  inv_all; subst. simpl in *.
+  Check Ap_pctxD.
+  gather_facts.
+  eapply Pure_pctxD; eauto.
+  intros.
+  specialize (H7 _ _ H8).
+  destruct H7 as [? ?]. specialize (H15 HList.Hnil). simpl in H15.
+  rewrite H15; clear H15.
+  unfold field_lookup. exists c; split; [|reflexivity].
+  autorewrite with exprD_rw in H3; [|apply _];
+  simpl in H2; forward; inv_all; subst.
+  simpl.
+  unfold eq_rect_r. simpl.
+  
+  Require Import ExtLib.Data.String.
+  
+  Lemma class_lookup_sound s p c (H : class_lookup s p = Some c) : In (s, c) (p_classes p).
+  Proof.
+    destruct p. induction p_classes; simpl in *.
+    * unfold class_lookup in H. simpl in H; congruence.
+    * unfold class_lookup in H. simpl in H.
+      destruct a; simpl in *. consider (s ?[ eq ] s0); intros; subst.
+      + left. rewrite rel_dec_eq_true in H; inv_all; subst; [reflexivity| apply _|reflexivity].
+      + right. rewrite rel_dec_neq_false in H; [apply IHp_classes; apply H | apply _ | apply H0].
+  Qed.
+  
+  apply class_lookup_sound.
+  apply H9.
+  apply _.
+Qed.
+*)
+End FieldLookup.
